coq/theories/assembly/ASMSyntax.v
@@ -2,8 +2,6 @@ From impboot Require Import utils.Core.
 Require Import impboot.utils.Words4Naive.
 Require Import coqutil.Word.Interface.
 Require Import coqutil.Word.Properties.
-Require Import Corelib.Program.Wf.
-Require Import Lia.
 
 Inductive reg :=
 | RAX (* ret val *)
@@ -47,100 +45,6 @@ Inductive instr :=
 | PutChar
 | Exit
   (* comment (has no semantics) *)
-| Comment (s: list ascii).
+| Comment (s: string).
 
 Notation asm := (list instr) (only parsing).
-
-Definition reg2str (r : reg) (s: string) : string :=
-  match r with
-  | RAX => "%rax"
-  | RDI => "%rdi"
-  | RBX => "%rbx"
-  | RBP => "%rbp"
-  | R12 => "%r12"
-  | R13 => "%r13"
-  | R14 => "%r14"
-  | R15 => "%r15"
-  | RDX => "%rdx"
-  end ++ s.
-
-Program Fixpoint num2str (n: nat) (s: string) {measure n}: string :=
-  if n <? 10 then String (ascii_of_nat (48 + n)) s
-  else num2str (n / 10) (String (ascii_of_nat (48 + (Nat.modulo n 10))) s).
-Next Obligation.
-  (* simpl.
-  specialize (Nat.divmod_spec n 9 0 9 ltac:(lia)) as ?.
-  destruct Nat.divmod eqn:?.
-  destruct H.
-  simpl. 
-  destruct n; simpl.
-  - destruct n0; try lia.
-    assert (n1 <> 9).
-    1: {
-      intros Hn1; subst.
-
-    }
-    lia. *)
-  admit.
-Admitted.
-
-Definition lab (n: nat) (s: string): string :=
-  String "L" (num2str n s).
-
-Fixpoint clean (cs: string) (acc: string): string :=
-  match cs with
-  | EmptyString => acc
-  | String c cs => if (nat_of_ascii c) <? 43 then clean cs acc else String c (clean cs acc)
-  end.
-
-Definition inst2str (i: instr) (s: string): string :=
-  match i with
-  | Const r imm => "movq $" ++ num2str (w2n imm) (", " ++ reg2str r s)
-  | Mov dst src => "movq " ++ reg2str src (", " ++ reg2str dst s)
-  | Add dst src => "addq " ++ reg2str src (", " ++ reg2str dst s)
-  | Sub dst src => "subq " ++ reg2str src (", " ++ reg2str dst s)
-  | Div r => "divq " ++ reg2str r s
-  | Jump Always n => "jmp " ++ lab n s
-  | Jump (Equal r1 r2) n =>
-      "cmpq " ++ reg2str r2 (", " ++ reg2str r1 (" ; je " ++ lab n s))
-  | Jump (Less r1 r2) n =>
-      "cmpq " ++ reg2str r2 (", " ++ reg2str r1 (" ; jb " ++ lab n s))
-  | Call n => "call " ++ lab n s
-  | Ret => "ret" ++ s
-  | Pop r => "popq " ++ reg2str r s
-  | Push r => "pushq " ++ reg2str r s
-  | Load_RSP r n => "movq " ++ num2str (8 * n) ("(%rsp), " ++ reg2str r s)
-  | Store_RSP r n => "movq " ++ num2str (8 * n) (reg2str r ("(%rsp), " ++ s))
-  | Add_RSP n => "addq $" ++ num2str (8 * n) (", %rsp" ++ s)
-  | Sub_RSP n => "subq $" ++ num2str (8 * n) (", %rsp" ++ s)
-  | Store src a w =>
-      "movq " ++ reg2str src (", " ++ num2str (w2n4 w) ("(" ++ reg2str a (")" ++ s)))
-  | Load dst a w =>
-      "movq " ++ num2str (w2n4 w) ("(" ++ reg2str a ("), " ++ reg2str dst s))
-  | GetChar => "movq stdin(%rip), %rdi ; call _IO_getc@PLT" ++ s
-  | PutChar => "movq stdout(%rip), %rsi ; call _IO_putc@PLT" ++ s
-  | Exit => "call exit@PLT" ++ s
-  | Comment c => "\n\n\t/* " ++ clean (string_of_list_ascii c) (" */" ++ s)
-  end.
-
-Fixpoint instrs2str (n: nat) (is: asm): string :=
-  match is with
-  | [] => EmptyString
-  | i :: is =>
-    lab n (String ":" (String "009" (inst2str i (String "010" (instrs2str (n+1) is)))))
-  end.
-
-Definition asm2str (is: asm): string := String.concat ""
-    ["\t.bss\n";
-     "\t.p2align 3          /* 8-byte align        */\n";
-     "heapS:\n";
-     "\t.space 8*1024*1024  /* bytes of heap space */\n";
-     "\t.p2align 3          /* 8-byte align        */\n";
-     "heapE:\n\n";
-     "\t.text\n";
-     "\t.globl main\n";
-     "main:\n";
-     "\tsubq $8, %rsp        /* 16-byte align %rsp */\n";
-     "\tmovabs $heapS, %r14  /* r14 := heap start  */\n";
-     "\tmovabs $heapE, %r15  /* r15 := heap end    */\n\n"]%string
-    ++ instrs2str 0 is.
